kore/src/Signature.v
@@ -12,8 +12,8 @@ Class Sorts := {
     sort_eqdec :: EqDecision sort;
     sort_countable :: Countable sort;
     subsort : CRelationClasses.crelation sort;
-    subsort_preo :: CRelationClasses.PreOrder subsort;
-    subsort_po :: CRelationClasses.PartialOrder eq subsort;
+(*     subsort_preo :: CRelationClasses.PreOrder subsort;
+    subsort_po :: CRelationClasses.PartialOrder eq subsort; *)
 }.
 
 Class Variables {Ss : Sorts} := {
