kore/src/theories/Baz.v
@@ -1,0 +1,336 @@
+From MatchingLogic Require Export stdpp_ext.
+From Kore Require Export Semantics.
+Import Signature.StringVariables.
+Import Kore.Syntax.Notations.
+
+From Coq Require Import ZArith.
+
+Open Scope kore_scope.
+Open Scope hlist_scope.
+Open Scope string_scope.
+
+Ltac autorewrite_set :=
+  repeat (
+    rewrite intersection_top_l_L +
+    rewrite intersection_top_r_L +
+    rewrite union_empty_l_L +
+    rewrite union_empty_r_L +
+    rewrite propset_difference_neg +
+    rewrite propset_union_simpl +
+    rewrite propset_intersection_simpl +
+    rewrite singleton_subseteq_l
+  ).
+
+Ltac basic_simplify_krule :=
+  simpl;
+  eval_helper;
+  repeat rewrite_app_ext;
+  autorewrite_set.
+Ltac simplify_krule :=
+  basic_simplify_krule;
+  apply propset_top_elem_of_2;
+  intro;
+  apply elem_of_PropSet;
+  repeat rewrite elem_of_PropSet;
+  repeat rewrite singleton_subseteq;
+  repeat rewrite singleton_eq.
+
+
+Ltac abstract_var := 
+  match goal with
+    | [|- context [evar_valuation ?σ ?s]] =>
+      let x := fresh "var" in
+      let Hx := fresh "Hvar" in
+        remember (evar_valuation σ s) as x eqn:Hx (*;
+        clear Hx;
+        revert x *)
+    end.
+
+Module T.
+
+  (* We have two sorts: natural numbers and bools *)
+  Inductive DemoSorts :=
+  | SortBaz
+  | SortBar
+  | SortFoo
+  | SortBax
+  (* | SortInt *)
+(*   | SortGeneratedCounterCell
+  | SortGeneratedTopCell *)
+  (* | SortList *)
+  | SortK
+  | SortKItem.
+
+  (* We prove decidable equality and finiteness of the type above. *)
+  Instance DemoSorts_eq_dec : EqDecision DemoSorts.
+  Proof. solve_decision. Defined.
+  Program Instance DemoSorts_finite : finite.Finite DemoSorts := {
+    enum := [SortBaz; SortBar; SortFoo; SortBax; (* SortInt; *)
+             (* SortGeneratedCounterCell; SortGeneratedTopCell; *)
+             (* SortList; *) SortK; SortKItem];
+  }.
+  Next Obligation. compute_done. Defined.
+  Final Obligation. destruct x; set_solver. Defined.
+
+
+  Inductive DemoSyms :=
+  | SymBar
+  | SymBaz1
+  | SymBaz2
+  | SymBax
+  | SymF
+  | SymKseq
+  | SymDotk.
+
+  (* We prove decidable equality and finiteness of the type above. *)
+  Instance DemoSyms_eq_dec : EqDecision DemoSyms.
+  Proof. solve_decision. Defined.
+  Program Instance DemoSyms_finite : finite.Finite DemoSyms := {
+    enum := [SymBar; SymBaz1; SymBaz2; SymBax; SymF; SymKseq; SymDotk];
+  }.
+  Next Obligation. compute_done. Defined.
+  Final Obligation. destruct x; set_solver. Defined.
+
+  Inductive Demo_subsort : CRelationClasses.crelation DemoSorts :=
+  | inj_bax_kitem : Demo_subsort SortBax SortKItem
+  | inj_foo_kitem : Demo_subsort SortFoo SortKItem
+  | inj_baz_kitem : Demo_subsort SortBaz SortKItem
+  | inj_bar_kitem : Demo_subsort SortBar SortKItem
+  | inj_bax_foo : Demo_subsort SortBax SortFoo
+  | inj_baz_foo : Demo_subsort SortBaz SortFoo
+  | inj_bar_foo : Demo_subsort SortBar SortFoo
+  | inj_baz_bar : Demo_subsort SortBaz SortBar
+  | inj_baz_bax : Demo_subsort SortBaz SortBax.
+
+  Goal
+    forall s1 s2 s3, Demo_subsort s1 s2 -> Demo_subsort s2 s3 ->
+      Demo_subsort s1 s3.
+  Proof.
+    intros ??? H1 H2; inversion H1; inversion H2; try constructor; subst; try discriminate.
+  Defined.
+
+  Goal
+    forall s1 s2, Demo_subsort s1 s2 -> Demo_subsort s2 s1 -> s1 = s2.
+  Proof.
+    intros; inversion H; subst; inversion H0; subst.
+  Defined.
+
+  (* In the signature, we need to define the sorts, the variable types,
+     and the typing/sorting rules for symbols: *)
+  Program Instance DemoSignature : Signature := {|
+    sorts := {|
+      sort := DemoSorts;
+      subsort := Demo_subsort
+    |};
+    variables := StringVariables;
+    symbols := {|
+      symbol := DemoSyms;
+      arg_sorts :=
+        fun σ => match σ with
+                  | SymBar => []
+                  | SymBaz1 => []
+                  | SymBaz2 => []
+                  | SymBax => []
+                  | SymF => [SortFoo]
+                  | SymKseq => [SortKItem; SortK]
+                  | SymDotk => []
+                 end;
+      ret_sort := fun σ => match σ with
+                            | SymBar => SortBar
+                            | SymBaz1 => SortBaz
+                            | SymBaz2 => SortBaz
+                            | SymBax => SortBax
+                            | SymF => SortBaz
+                            | SymKseq => SortK
+                            | SymDotk => SortK
+                           end;
+    |};
+  |}.
+
+  Lemma neqs_eq {A} {a b : A} (p q : a ≠ b) : p = q.
+  Proof.
+    apply functional_extensionality. intros. destruct (p x).
+  Defined.
+
+  (* Lemma subsort_unique {s1 s2} (p1 p2 : Demo_subsort s1 s2) : p1 = p2. *)
+  (* Proof. *)
+  (*   dependent induction p1; dependent destruction p2. *)
+  (*   reflexivity. *)
+  (*   destruct n0. reflexivity. *)
+  (*   destruct n0. reflexivity. *)
+  (*   f_equal; apply neqs_eq. *)
+  (* Defined. *)
+
+  (* Instance carrier_eqdec A : EqDecision (carrier A). *)
+  (* Proof. *)
+  (*   unfold EqDecision, Decision. *)
+  (*   (1* No induction principle if the type appears in another *1) *)
+  (*   (1* type (list here). As usual... *1) *)
+  (*   revert A. fix IH 2. *)
+  (*   intros. *)
+  (*   dependent destruction x; dependent destruction y; try ((right; discriminate) + (left; reflexivity)). *)
+  (*   * destruct (decide (n = n0)) as [-> | ?]; [left; reflexivity | right; congruence]. *)
+  (*   * destruct (decide (b = b0)) as [-> | ?]; [left; reflexivity | right; congruence]. *)
+  (*   * pose proof @list_eq_dec _ (IH SortKItem) l l0 as [-> | ?]; [left; reflexivity | right; congruence]. *)
+  (*     Guarded. *)
+  (*   * destruct (decide (s0 = s1)) as [-> | ?]. *)
+  (*     - destruct (IH _ x y) as [-> | ?]. *)
+  (*       + rewrite (subsort_unique P P0); by left. *)
+  (*       + right. intro. inversion H. inversion_sigma H2. *)
+  (*         rewrite <- Eqdep.EqdepTheory.eq_rect_eq in H2_0. *)
+  (*         congruence. *)
+  (*     - right. intro. inversion H. congruence. *)
+  (* Qed. *)
+
+  Definition inb {A} {_ : EqDecision A} (x : A) (xs : list A) : bool.
+  Proof.
+    induction xs. exact false.
+    exact (if decide (x = a) then true else false).
+  Defined.
+
+  Inductive baz_carrier : Set :=
+  | c_baz1
+  | c_baz2
+  with bar_carrier : Set :=
+  | c_bar
+  | c_inj_baz_bar (b : baz_carrier)
+  with bax_carrier : Set :=
+  | c_bax
+  | c_inj_baz_bax (b : baz_carrier)
+  with foo_carrier : Set :=
+  | c_inj_bar_foo (b : bar_carrier)
+  | c_inj_bax_foo (b : bax_carrier)
+  | c_inj_baz_foo (b : baz_carrier)
+  with k_carrier : Set  :=
+  | c_dotk
+  | c_kseq (k : kitem_carrier) (l : k_carrier)
+  with kitem_carrier : Set :=
+  | c_inj_bar_kitem (b : bar_carrier)
+  | c_inj_bax_kitem (b : bax_carrier)
+  | c_inj_baz_kitem (b : baz_carrier)
+  | c_inj_foo_kitem (b : foo_carrier)
+  .
+
+  Definition carrier (s : DemoSorts) : Set :=
+  match s with
+  | SortBaz => baz_carrier
+  | SortBar => bar_carrier
+  | SortFoo => foo_carrier
+  | SortBax => bax_carrier
+  | SortK => k_carrier
+  | SortKItem => kitem_carrier
+  end.
+
+  Definition f (x : foo_carrier) : baz_carrier :=
+  match x with (* This pattern matching is retr of klean! *)
+  | c_inj_bar_foo _ => c_baz1
+  | c_inj_baz_foo _ => c_baz1
+  | _ => c_baz2
+  end.
+
+  Program Definition DemoModel : @Model DemoSignature := mkModel_singleton
+    carrier
+    (fun σ =>
+        match σ with
+        | SymBar => c_bar
+        | SymBaz1 => c_baz1
+        | SymBaz2 => c_baz2
+        | SymBax => c_bax
+        | SymF => f
+        | SymKseq => c_kseq
+        | SymDotk => c_dotk
+        end
+      )
+    _
+    _.
+  Next Obligation.
+    destruct s; repeat constructor.
+  Defined.
+  Final Obligation.
+    destruct s1, s2; simpl; intros H x; inversion H; subst.
+    * exact (c_inj_baz_bar x).
+    * exact (c_inj_baz_foo x).
+    * exact (c_inj_baz_bax x).
+    * exact (c_inj_baz_kitem x).
+    * exact (c_inj_bar_foo x).
+    * exact (c_inj_bar_kitem x).
+    * exact (c_inj_foo_kitem x).
+    * exact (c_inj_bax_foo x).
+    * exact (c_inj_bax_kitem x).
+  Defined.
+
+  Search fmap "set".
+
+  Lemma fmap_set_singleton :
+    forall {A B : Type}
+      (f : A -> B) (x : A),
+      f <$> ({[x]} : propset A) = ({[f x]} : propset B).
+  Proof.
+    set_solver.
+  Defined.
+
+  Goal
+    forall ρ, @eval DemoSignature DemoModel [] [] _ ρ
+      (SymF ⋅ ⟨kore_inj _ inj_bar_foo (SymBar ⋅ ⟨⟩) ⟩) = {[c_baz1]}.
+  Proof.
+    intros.
+    rewrite eval_app_simpl. simpl.
+    rewrite eval_equation_21. simpl.
+    rewrite (@eval_app_simpl DemoSignature _ _ _ SymBar).
+    simpl hmap.
+    rewrite_app_ext.
+    rewrite fmap_set_singleton.
+    rewrite_app_ext.
+    reflexivity.
+  Qed.
+
+  Goal
+    forall ρ, @eval DemoSignature DemoModel [] [] _ ρ
+      (SymF ⋅ ⟨kore_inj _ inj_baz_foo (SymBaz2 ⋅ ⟨⟩) ⟩) = {[c_baz1]}.
+  Proof.
+    intros.
+    rewrite eval_app_simpl. simpl.
+    rewrite eval_equation_21. simpl.
+    rewrite (@eval_app_simpl DemoSignature _ _ _ SymBaz2).
+    simpl hmap.
+    rewrite_app_ext.
+    rewrite fmap_set_singleton.
+    rewrite_app_ext.
+    reflexivity.
+  Qed.
+
+  Goal
+    forall ρ, @eval DemoSignature DemoModel [] [] _ ρ
+      (SymF ⋅ ⟨kore_inj _ inj_bar_foo (kore_inj _ inj_baz_bar (SymBaz2 ⋅ ⟨⟩)) ⟩) = {[c_baz1]}.
+  Proof.
+    intros.
+    rewrite eval_app_simpl. simpl.
+    rewrite eval_equation_21. simpl.
+    rewrite eval_equation_21. simpl.
+    rewrite (@eval_app_simpl DemoSignature _ _ _ SymBaz2).
+    simpl hmap.
+    rewrite_app_ext.
+    rewrite fmap_set_singleton.
+    rewrite fmap_set_singleton.
+    rewrite_app_ext.
+    reflexivity.
+  Qed.
+
+  Goal
+    forall ρ, @eval DemoSignature DemoModel [] [] _ ρ
+      (SymF ⋅ ⟨kore_inj _ inj_bax_foo (kore_inj _ inj_baz_bax (SymBaz2 ⋅ ⟨⟩)) ⟩) = {[c_baz1]}.
+  Proof.
+    intros.
+    rewrite eval_app_simpl. simpl.
+    rewrite eval_equation_21. simpl.
+    rewrite eval_equation_21. simpl.
+    rewrite (@eval_app_simpl DemoSignature _ _ _ SymBaz2).
+    simpl hmap.
+    rewrite_app_ext.
+    rewrite fmap_set_singleton.
+    rewrite fmap_set_singleton.
+    rewrite_app_ext.
+    Fail reflexivity.
+  Abort.
+
+End T.
